unfold casts

pulse/Pulse.Lib.C.Casts.Bool.fsti
@@ -1,20 +1,20 @@
 module Pulse.Lib.C.Casts.Bool
 
-let bool_to_int (b:bool) = if b then 1 else 0
-let bool_to_int64 (b:bool) = if b then 1L else 0L
-let bool_to_uint64 (b:bool) = if b then 1UL else 0UL
-let bool_to_int32 (b:bool) = if b then 1l else 0l
-let bool_to_uint32 (b:bool) = if b then 1ul else 0ul
-let bool_to_int16 (b:bool) = if b then 1s else 0s
-let bool_to_uint16 (b:bool) = if b then 1us else 0us
-let bool_to_int8 (b:bool) = if b then 1y else 0y
-let bool_to_uint8 (b:bool) = if b then 1uy else 0uy
+unfold let bool_to_int (b:bool) = if b then 1 else 0
+unfold let bool_to_int64 (b:bool) = if b then 1L else 0L
+unfold let bool_to_uint64 (b:bool) = if b then 1UL else 0UL
+unfold let bool_to_int32 (b:bool) = if b then 1l else 0l
+unfold let bool_to_uint32 (b:bool) = if b then 1ul else 0ul
+unfold let bool_to_int16 (b:bool) = if b then 1s else 0s
+unfold let bool_to_uint16 (b:bool) = if b then 1us else 0us
+unfold let bool_to_int8 (b:bool) = if b then 1y else 0y
+unfold let bool_to_uint8 (b:bool) = if b then 1uy else 0uy
 
-let int8_to_bool (i:Int8.t) = Int8.ne i 0y
-let int16_to_bool (i:Int16.t) = Int16.ne i 0s
-let int32_to_bool (i:Int32.t) = Int32.ne i 0l
-let int64_to_bool (i:Int64.t) = Int64.ne i 0L
-let uint8_to_bool (i:UInt8.t) = UInt8.ne i 0uy
-let uint16_to_bool (i:UInt16.t) = UInt16.ne i 0us
-let uint32_to_bool (i:UInt32.t) = UInt32.ne i 0ul
-let uint64_to_bool (i:UInt64.t) = UInt64.ne i 0UL
+unfold let int8_to_bool (i:Int8.t) = Int8.ne i 0y
+unfold let int16_to_bool (i:Int16.t) = Int16.ne i 0s
+unfold let int32_to_bool (i:Int32.t) = Int32.ne i 0l
+unfold let int64_to_bool (i:Int64.t) = Int64.ne i 0L
+unfold let uint8_to_bool (i:UInt8.t) = UInt8.ne i 0uy
+unfold let uint16_to_bool (i:UInt16.t) = UInt16.ne i 0us
+unfold let uint32_to_bool (i:UInt32.t) = UInt32.ne i 0ul
+unfold let uint64_to_bool (i:UInt64.t) = UInt64.ne i 0UL
